src/program_proof/pav/evidence.v
@@ -1,0 +1,50 @@
+From Perennial.program_proof Require Import grove_prelude.
+From Goose.github_com.mit_pdos.pav Require Import kt.
+
+From Perennial.program_proof.pav Require Import core cryptoffi serde.
+
+Module Evid.
+Record t :=
+  mk {
+    sigDig0: SigDig.t;
+    sigDig1: SigDig.t;
+  }.
+Section defs.
+Context `{!heapGS Σ, !pavG Σ}.
+Definition own ptr obj : iProp Σ :=
+  ∃ ptr_sigDig0 ptr_sigDig1,
+  "Hown_sigDig0" ∷ SigDig.own ptr_sigDig0 obj.(sigDig0) ∗
+  "Hptr_sigDig0" ∷ ptr ↦[Evid :: "sigDig0"] #ptr_sigDig0 ∗
+  "Hown_sigDig1" ∷ SigDig.own ptr_sigDig1 obj.(sigDig1) ∗
+  "Hptr_sigDig1" ∷ ptr ↦[Evid :: "sigDig1"] #ptr_sigDig1.
+End defs.
+End Evid.
+
+Section defs.
+Context `{!heapGS Σ, !pavG Σ}.
+
+Definition is_SigDig obj pk : iProp Σ :=
+  is_sig pk (PreSigDig.encodesF (PreSigDig.mk obj.(SigDig.Epoch) obj.(SigDig.Dig))) obj.(SigDig.Sig).
+
+Definition is_Evid obj pk : iProp Σ :=
+  "His_sigDig0" ∷ is_SigDig obj.(Evid.sigDig0) pk ∗
+  "His_sigDig1" ∷ is_SigDig obj.(Evid.sigDig1) pk.
+End defs.
+
+Section wps.
+Context `{!heapGS Σ, !pavG Σ}.
+
+Lemma wp_CheckSigDig ptr obj sl_pk pk :
+  {{{
+    "Hown_SigDig" ∷ SigDig.own ptr obj ∗
+    "#Hsl_pk" ∷ own_slice_small sl_pk byteT DfracDiscarded pk
+  }}}
+  CheckSigDig #ptr (slice_val sl_pk)
+  {{{
+    (err : bool), RET #err;
+    "Hown_SigDig" ∷ SigDig.own ptr obj ∗
+    "Hgenie" ∷ (is_SigDig obj pk ∗-∗ ⌜ err = false ⌝)
+  }}}.
+Proof. Admitted.
+
+End wps.
